aneris/examples/reliable_communication/lib/repdb/spec/ras.v
@@ -1,0 +1,29 @@
+From iris.algebra Require Import auth gmap excl excl_auth.
+From aneris.algebra Require Import monotone.
+From aneris.aneris_lang.lib Require Import lock_proof.
+From aneris.examples.reliable_communication.lib.repdb.spec
+     Require Import db_params time events resources.
+
+
+Class DBG `{!DB_time, !DB_events} Σ :=
+  {
+    DBG_Global_mem_excl :>
+      inG Σ (authUR (gmapUR Key (prodR fracR (agreeR (optionO (leibnizO we))))));
+    DBG_Global_history_mono :>
+      inG Σ (authUR (monotoneUR (@prefix (leibnizO we))));
+    DBG_Local_history_mono :>
+      inG Σ (authUR (gmapUR socket_address
+                               (monotoneUR (@prefix (leibnizO we)))));
+    DBG_lockG :>
+      lockG Σ;
+}.
+
+Definition DBΣ `{!DB_time, !DB_events} : gFunctors :=
+  #[GFunctor (authUR (gmapUR Key (prodR fracR (agreeR (optionO (leibnizO we))))));
+    GFunctor (authUR (monotoneUR (@prefix (leibnizO we))));
+    GFunctor (authUR (gmapUR socket_address
+                               (monotoneUR (@prefix (leibnizO we)))));
+    lockΣ].
+
+Instance subG_DBΣ `{!DB_time, !DB_events, !lockG Σ} : subG DBΣ Σ → DBG Σ.
+Proof. solve_inG. Qed.
